<?xml version="1.0" encoding="UTF-8"?>

<!DOCTYPE rdfs [
	<!ENTITY rdf "http://www.w3.org/1999/02/22-rdf-syntax-ns#">
	<!ENTITY rdfs "http://www.w3.org/2000/01/rdf-schema#">
	<!ENTITY dc "http://purl.org/dc/elements/1.1/">
	<!ENTITY dct "http://purl.org/dc/terms/">
	<!ENTITY foaf "http://xmlns.com/foaf/0.1/">
	<!ENTITY owl "http://www.w3.org/2002/07/owl#">
]>

<rdf:RDF xml:base="http://www.w3.org/2004/02/skos/core" xmlns:xml="http://www.w3.org/XML/1998/namespace" xmlns:rdf="http://www.w3.org/1999/02/22-rdf-syntax-ns#" xmlns:rdfs="http://www.w3.org/2000/01/rdf-schema#" xmlns:dc="http://purl.org/dc/elements/1.1/" xmlns:dct="http://purl.org/dc/terms/" xmlns:owl="http://www.w3.org/2002/07/owl#">
	
	<!-- Description of this schema -->
	
	<rdf:Description rdf:about="">
		<dc:title>SKOS-Core 1.0</dc:title>
		<dc:description>An RDF schema for encoding simple concept schemes such as thesauri, taxonomies and subject heading schemes.</dc:description>
		<dc:creator>Alistair Miles</dc:creator>
		<dc:creator>Nikki Rogers</dc:creator>
		<dc:creator>Dave Beckett</dc:creator>
		<rdfs:seeAlso rdf:resource=""/>
		<dct:modified/>
	</rdf:Description>
	
	<!-- Fundamental classes -->

	<rdfs:Class rdf:ID="ConceptScheme">
		<rdfs:label>Concept-Scheme</rdfs:label>
		<rdfs:comment>A concept scheme is any collection of concepts forming a coherent scheme, e.g. a thesaurus or a set of subject headings.</rdfs:comment>
	</rdfs:Class>
	
	<rdfs:Class rdf:ID="Concept">
		<rdfs:label>Concept</rdfs:label>
		<rdfs:comment>Use this class to indicate that a node is an abstract concept.  The concept may be part of some conceptual scheme such as a thesaurus.</rdfs:comment>
	</rdfs:Class>
		
	<!-- Basic properties of concepts -->

	<rdf:Property rdf:ID="inScheme">
		<rdfs:label>in-scheme</rdfs:label>
		<rdfs:subPropertyOf rdf:resource="http://www.w3.org/2000/01/rdf-schema#isDefinedBy"/>
		<rdfs:domain rdf:resource="#Concept"/>
		<rdfs:range rdf:resource="#ConceptScheme"/>
		<rdfs:comment>Use this property to state that a concept is a part of some concept scheme.  A concept may be a part of more than one scheme.</rdfs:comment>
	</rdf:Property>
	
	<rdf:Property rdf:ID="prefLabel">
		<rdfs:label>preferred-label</rdfs:label>
		<rdfs:subPropertyOf rdf:resource="http://www.w3.org/2000/01/rdf-schema#label"/>
		<rdfs:comment>Use this property to indicate a preferred label for a resource.  If the resource is a concept in some conceptual scheme, then it is recommended that the preferred label be a unique label within that scheme.</rdfs:comment>
	</rdf:Property>
	
	<rdf:Property rdf:ID="altLabel">
		<rdfs:label>alternative-label</rdfs:label>
		<rdfs:subPropertyOf rdf:resource="http://www.w3.org/2000/01/rdf-schema#label"/>
		<rdfs:comment>Use this property to indicate an alternative (non-preferred) label for a resource.</rdfs:comment>
	</rdf:Property>

	<rdf:Property rdf:ID="prefSymbol">
		<rdfs:label>preferred-symbol</rdfs:label>
		<rdfs:domain rdf:resource="http://www.w3.org/1999/02/22-rdf-syntax-ns#Resource"/>
		<rdfs:range rdf:resource="http://xmlns.com/foaf/0.1/Image"/>
		<rdfs:comment>Use this property to indicate a preferred symbolic representation for a resource.</rdfs:comment>
	</rdf:Property>
	
	<rdf:Property rdf:ID="altSymbol">
		<rdfs:label>alternative-symbol</rdfs:label>
		<rdfs:domain rdf:resource="http://www.w3.org/1999/02/22-rdf-syntax-ns#Resource"/>
		<rdfs:range rdf:resource="http://xmlns.com/foaf/0.1/Image"/>
		<rdfs:comment>Use this property to indicate an alternative (non-preferred) symbolic representation for a resource.</rdfs:comment>
	</rdf:Property>

	<rdf:Property rdf:ID="externalID">
		<rdfs:label>external-identifier</rdfs:label>
		<rdfs:subPropertyOf rdf:resource="http://www.w3.org/1999/02/22-rdf-syntax-ns#value"/>
		<rdfs:domain rdf:resource="#Concept"/>
		<rdfs:comment>Use or extend this property to indicate any non-URI code that is used to uniquely identify a concept within a conceptual scheme.</rdfs:comment>
	</rdf:Property>
	
	<rdf:Property rdf:ID="semanticRelation">
		<rdfs:label>semantic-relation</rdfs:label>
		<rdfs:domain rdf:resource="#Concept"/>
		<rdfs:range rdf:resource="#Concept"/>
		<rdfs:comment>This is the super-property of all properties used to make statements about how concepts within the same conceptual scheme relate to each other.</rdfs:comment>
	</rdf:Property>
	
	<!-- Generic semantic relation properties -->
	
	<rdf:Property rdf:ID="broader">
		<rdfs:label>has-broader</rdfs:label>
		<rdf:type rdf:resource="http://www.w3.org/2002/07/owl#TransitiveProperty"/>
		<rdfs:subPropertyOf rdf:resource="#semanticRelation"/>
		<rdfs:comment>This property carries weak semantics.  It may be used to state that the object is in some way more general in meaning than the subject.  Essentially it provides a means of organising concepts into hierarchical structures, without being restrictive about the exact semantic implications of the hierarchical structure itself.  Extend this property to create properties that carry stronger semantics, but may be reduced to a hierarchical structure for simple visual displays.</rdfs:comment>
	</rdf:Property>
	
	<rdf:Property rdf:ID="narrower">
		<rdfs:label>has-narrower</rdfs:label>
		<rdf:type rdf:resource="http://www.w3.org/2002/07/owl#TransitiveProperty"/>
		<rdfs:subPropertyOf rdf:resource="#semanticRelation"/>
		<owl:inverseOf rdf:resource="#broader"/>
		<rdfs:comment>This property is the inverse of the 'broader' property.</rdfs:comment>
	</rdf:Property>
	
	<rdf:Property rdf:ID="related">
		<rdfs:label>related-to</rdfs:label>
		<rdfs:subPropertyOf rdf:resource="#semanticRelation"/>
		<rdfs:comment>This property carries weak semantics.  It may be used to state that that the object is in some way related to the subject, and the nature of that relationship is NOT to be treated as hierarchical.  Extend this property to create properties with stronger semantics, but may still be reduced to an associative structure for simple visual display.</rdfs:comment>
	</rdf:Property>
	
	<!-- Semantic relation property extensions -->
	
	<rdf:Property rdf:ID="broaderInstantive">
		<rdfs:label>instance-of</rdfs:label>
		<rdfs:subPropertyOf rdf:resource="#broader"/>
		<rdfs:subPropertyOf rdf:resource="http://www.w3.org/1999/02/22-rdf-syntax-ns#type"/>
		<rdfs:comment>An extension of the 'broader' property to specify the instantiation relationship between two concepts.  This property is semantically equivalent to the 'rdf:type' property.</rdfs:comment>
	</rdf:Property>
	
	<rdf:Property rdf:ID="narrowerInstantive">
		<rdfs:label>has-instance</rdfs:label>
		<rdfs:subPropertyOf rdf:resource="#narrower"/>
		<owl:inverseOf rdf:resource="#broaderInstantive"/>
		<rdfs:comment>An extension of the 'narrower' property to specify the instantiation relationship between two concepts.</rdfs:comment>
	</rdf:Property>
	
	<rdf:Property rdf:ID="broaderGeneric">
		<rdfs:label>sub-class-of</rdfs:label>
		<rdf:type rdf:resource="http://www.w3.org/2002/07/owl#TransitiveProperty"/>
		<rdfs:subPropertyOf rdf:resource="#broader"/>
		<rdfs:subPropertyOf rdf:resource="http://www.w3.org/2000/01/rdf-schema#subClassOf"/>
		<rdfs:comment>An extension of the 'broader' property to specify the class subsumption relationship between two concepts.  This property is semantically equivalent to the 'rdfs:subClassOf' property.</rdfs:comment>
	</rdf:Property>
	
	<rdf:Property rdf:ID="narrowerGeneric">
		<rdfs:label>super-class-of</rdfs:label>
		<rdf:type rdf:resource="http://www.w3.org/2002/07/owl#TransitiveProperty"/>
		<rdfs:subPropertyOf rdf:resource="#narrower"/>
		<owl:inverseOf rdf:resource="#broaderGeneric"/>
		<rdfs:comment>An extension of the 'narrower' property to specify the class subsumption relationship between two concepts.  This property should be considered the inverse of 'broaderGeneric'.</rdfs:comment>
	</rdf:Property>
	
	<rdf:Property rdf:ID="broaderPartitive">
		<rdfs:label>part-of</rdfs:label>
		<rdf:type rdf:resource="http://www.w3.org/2002/07/owl#TransitiveProperty"/>
		<rdfs:subPropertyOf rdf:resource="#broader"/>
		<rdfs:subPropertyOf rdf:resource="http://purl.org/dc/terms/isPartOf"/>
		<rdfs:comment>An extension of the 'broader' property to specify a partitive relationship between two concepts.</rdfs:comment>
	</rdf:Property>
	
	<rdf:Property rdf:ID="narrowerPartitive">
		<rdfs:label>has-part</rdfs:label>
		<rdf:type rdf:resource="http://www.w3.org/2002/07/owl#TransitiveProperty"/>
		<rdfs:subPropertyOf rdf:resource="#narrower"/>
		<rdfs:subPropertyOf rdf:resource="http://purl.org/dc/terms/hasPart"/>
		<owl:inverseOf rdf:resource="#broaderPartitive"/>
		<rdfs:comment>An extension of the 'narrower' property to specify a partitive relationship between two concepts.  This property should be considered to be the inverse of 'broaderPartitive'.</rdfs:comment>
	</rdf:Property>

	<rdf:Property rdf:ID="relatedPartOf">
		<rdfs:label>part-of</rdfs:label>
		<rdf:type rdf:resource="http://www.w3.org/2002/07/owl#TransitiveProperty"/>
		<rdfs:subPropertyOf rdf:resource="#related"/>
		<rdfs:subPropertyOf rdf:resource="http://purl.org/dc/terms/isPartOf"/>
		<rdfs:comment>An extension of the 'related' property.  Use this property to express a partitive relationship between concepts, where it is desired that such a relationship be treated as associative and NOT hierarchical.</rdfs:comment>
	</rdf:Property>

	<rdf:Property rdf:ID="relatedHasPart">
		<rdfs:label>has-part</rdfs:label>
		<rdf:type rdf:resource="http://www.w3.org/2002/07/owl#TransitiveProperty"/>
		<rdfs:subPropertyOf rdf:resource="#related"/>
		<rdfs:subPropertyOf rdf:resource="http://purl.org/dc/terms/hasPart"/>
		<rdfs:comment>An extension of the 'related' property.  This property should be treated as the inverse of 'relatedPartOf'.</rdfs:comment>
	</rdf:Property>

	<rdf:Property rdf:ID="relatedSymmetric">
		<rdfs:label>related</rdfs:label>
		<rdf:type rdf:resource="http://www.w3.org/2002/07/owl#SymmetricProperty"/>
		<rdfs:subPropertyOf rdf:resource="#related"/>
		<rdfs:comment>An extension of the 'related' property to be used where the relationship can be treated as being symmetric.</rdfs:comment>
	</rdf:Property>
	

	<!-- Scope and other notes -->
	
	<rdf:Property rdf:ID="scopeNote">
		<rdfs:label>scope-note</rdfs:label>
		<rdfs:subPropertyOf rdf:resource="http://www.w3.org/2000/01/rdf-schema#comment"/>
		<rdfs:comment>A scope note is a piece of text that in some way helps to elucidate the intended meaning of a concept.</rdfs:comment>
		<rdfs:domain rdf:resource="#Concept"/>
	</rdf:Property>
	
	<rdf:Property rdf:ID="definition">
		<rdfs:label>definition</rdfs:label>
		<rdfs:subPropertyOf rdf:resource="http://www.w3.org/2000/01/rdf-schema#comment"/>
		<rdfs:comment>A formal definition of the intended meaning of a concept.</rdfs:comment>
		<rdfs:domain rdf:resource="#Concept"/>
	</rdf:Property>
	
	<rdf:Property rdf:ID="example">
		<rdfs:label>example</rdfs:label>
		<rdfs:subPropertyOf rdf:resource="http://www.w3.org/2000/01/rdf-schema#comment"/>
		<rdfs:comment>A contextual example of the use of a concept, that helps to elucidate its intended meaning.</rdfs:comment>
		<rdfs:domain rdf:resource="#Concept"/>
	</rdf:Property>
	
</rdf:RDF>