<?xml version="1.0" encoding="iso-8859-1"?>

<!DOCTYPE owl [
  <!ENTITY rdf  "http://www.w3.org/1999/02/22-rdf-syntax-ns#">
  <!ENTITY rdfs "http://www.w3.org/2000/01/rdf-schema#">
  <!ENTITY owl  "http://www.w3.org/2002/07/owl#">
  <!ENTITY xsd  "http://www.w3.org/2000/10/XMLSchema#">
  <!ENTITY dc   "http://purl.org/dc/elements/1.1/">
  <!ENTITY tool "http://www.swi.psy.uva.nl/mia/tool#">
]>

<rdf:RDF
  xml:base  ="http://www.swi.psy.uva.nl/mia/tool"
  xmlns:rdf ="&rdf;"
  xmlns:rdfs="&rdfs;"
  xmlns:owl ="&owl;"
  xmlns:xsd ="&xsd;"
  xmlns:dc  ="&dc;"
  xmlns:tool="&tool;"
>

<!--
<Ontology rdf:about="">
</Ontology>
-->

<rdfs:Class rdf:ID="&tool;Render">
  <rdfs:subClassOf rdf:resource="&rdfs;Resource"/>
  <rdfs:label>Render</rdfs:label>
  <rdfs:comment>Specifies how this class is rendered in the SWI-Prolog/XPCE
                RDFS browser.
  </rdfs:comment>
</rdfs:Class>

<rdf:Property rdf:about="&tool;context">
  <rdfs:label>context</rdfs:label>
  <rdfs:comment>Denotes the XPCE class of the container that must render
                a individual of this Class.
  </rdfs:comment>
  <rdfs:domain rdf:resource="&tool;Render"/>
  <rdfs:range  rdf:resource="&rdfs;Literal"/>
</rdf:Property>

<rdf:Property rdf:about="&tool;role">
  <rdfs:label>role</rdfs:label>
  <rdfs:comment>Role (triple field) of the visualisation
  </rdfs:comment>
  <rdfs:domain rdf:resource="&tool;Render"/>
  <rdfs:range  rdf:resource="&rdfs;Literal"/>
</rdf:Property>

<rdf:Property rdf:about="&tool;class">
  <rdfs:label>class</rdfs:label>
  <rdfs:comment>Denotes the XPCE object used to render an individual
                of this Class.
  </rdfs:comment>
  <rdfs:domain rdf:resource="&tool;Render"/>
  <rdfs:range  rdf:resource="&rdfs;Literal"/>
</rdf:Property>

<rdf:Property rdf:about="&tool;domain">
  <rdfs:label>domain</rdfs:label>
  <rdfs:comment>The root of the class hierarchy this rendering
                applies too.
  </rdfs:comment>
  <rdfs:domain rdf:resource="&tool;Render"/>
  <rdfs:range  rdf:resource="&rdfs;Class"/>
</rdf:Property>

</rdf:RDF>
